進捗

ProgrammingHaskell/Chapter05/LawfulSection5.lean
@@ -21,6 +21,8 @@ namespace LowerLetter
 end LowerLetter
 
 
+#eval (3 : UInt32) % 2
+
 namespace LowerLetter
   -- ## `UInt32` から `LowerLetter` への変換を行う関数
 
@@ -74,11 +76,21 @@ namespace LowerLetter
     exact UInt32.le_iff_toNat_le
 
   theorem _root_.UInt32.ofNat_le_iff {m n : Nat} (hm : m < UInt32.size) (hn : n < UInt32.size)
-    : UInt32.ofNat m ≤ UInt32.ofNat n ↔ m ≤ n := by
-    sorry
+      : UInt32.ofNat m ≤ UInt32.ofNat n ↔ m ≤ n := by
+    rw [UInt32.le_iff_toNat_le]
+    simp only [UInt32.toNat_ofNat]
+    rw [Nat.mod_eq_of_lt hm]
+    rw [Nat.mod_eq_of_lt hn]
 
   /-- `Nat`から`LowerLetter`への範囲証明付きの変換 -/
-  def ofNat (n : Nat) (hn : n ≥ 97 && n ≤ 122) : LowerLetter :=
+  def ofNat (n : Nat) (hn : n ≥ 97 && n ≤ 122) : LowerLetter := by
+    replace hn : 97 ≤ n ∧ n ≤ 122 := by simpa using hn
+    dsimp [LowerLetter]
+    let u := UInt32.ofNat' n (by simp only [UInt32.size]; omega)
+    have hu : u ≥ 97 && u ≤ 122 := by
+      simp [u]
+
+      sorry
     sorry
 
 end LowerLetter
